\achapter

% 1
\answer $(b) A=\begin{bmatrix}
	1 & 0 \\	0 & -1
\end{bmatrix},\quad B=\begin{bmatrix}
	0 & e^{-i\alpha} \\ e^{i\alpha} & 0
\end{bmatrix}\quad $ $ (d) S=\dfrac{1}{\sqrt{2}}\begin{bmatrix}
	1 & 1 \\ e^{i\alpha} & -e^{i\alpha}
\end{bmatrix} $

 $ (e) A\rightarrow\begin{bmatrix}
	0 & 1 \\ 1 & 0
\end{bmatrix},\quad B\rightarrow\begin{bmatrix}
	1 & 0 \\ 0 & -1
\end{bmatrix} $

% 2
\answer $ B=\begin{bmatrix}
	0 & 0 \\ 0 & 1
\end{bmatrix},\quad A=\begin{bmatrix}
	0 & e^{i\alpha} \\ 0 & 0
\end{bmatrix} $

% 3
\answer $ U=\begin{bmatrix}
	\cos\omega e^{i\alpha} & \sin\omega e^{i\beta} \\
	-\sin\omega e^{-i\beta} & \cos\omega e^{-i\alpha}
\end{bmatrix} $

\stepcounter{answer}	\stepcounter{answer}	\stepcounter{answer}	\stepcounter{answer}	

% 8
\answer $ \dfrac{p^{2}}{2m}\phi(p)-\dfrac{1}{2}m\omega^{2}\hbar^{2}\dfrac{d^{2}}{dp^{2}}\phi(p)=E\phi(p) $

% 9
\answer $ \dfrac{p^{2}}{2m}\phi(p)-i\hbar F\dfrac{d}{dp}\phi(p)=E\phi(p),\quad \phi(p)=A\exp\left[\dfrac{i}{\hbar F}\left(E_{p}-\dfrac{p^{3}}{6m}\right)\right] $

\stepcounter{answer}	\stepcounter{answer}	\stepcounter{answer}	\stepcounter{answer}	\stepcounter{answer}

% 15
\answer $ \bar{x}=\sqrt{\dfrac{\hbar}{2\mu\omega}}(\alpha+\alpha^{*}),\quad \Delta x=\sqrt{\dfrac{\hbar}{2\mu\omega}} $

 $ \bar{p}=i(\alpha^{*}-\alpha)\sqrt{\dfrac{\mu\hbar\omega}{2}},\quad \Delta p=\sqrt{\dfrac{\mu\hbar\omega}{2}} $

 $ \bar{n}=\alpha^{*}\alpha,\quad \Delta n=\sqrt{\bar{n}} $

 $ \bar{E}=\left(\bar{n}+\dfrac{1}{2}\right)\hbar\omega,\quad \Delta E=\sqrt{\bar{n}}\hbar\omega $

% 16
\answer $ E_{n}=n-\dfrac{1}{3},\quad n=0,1,2,\cdots;\quad \varPsi_{0}(q)=ce^{-\frac{3q^{2}}{2}} $

\stepcounter{answer}	\stepcounter{answer}	\stepcounter{answer}	\stepcounter{answer}

% 21
\answer $\bar{J_{x}^{2}}=\bar{J_{y}^{2}}=(\Delta J_{x})^{2}=\hbar^{2}\dfrac{[j(j+1)-m^{2}]}{2} $

  不确定关系为$ \Delta J_{x}\Delta J_{y}\geqslant\dfrac{\hbar}{2}|\bar{J_{z}}|=\hbar\dfrac{|m|}{2} $

% 22
\answer $ \bar{J_{n}}=m\hbar\cos\theta $

% 23
\answer $ L_{x}=\dfrac{1}{\sqrt{2}}\begin{bmatrix}
	0 & 1 & 0 \\ 1 & 0 & 1 \\ 0 & 1 & 0 \\ 
\end{bmatrix},\quad L_{y}=\dfrac{1}{\sqrt{2}}\begin{bmatrix}
	0 & -i & 0 \\ i & 0 & -i \\ 0 & i & 0 \\ 
\end{bmatrix} $

% 24
\answer $ Y_{l,-l}=c(\sin\theta)^{l}e^{-il\varphi} $