\achapter
% \stepcounter{answer}

\stepcounter{answer}

% 2
\answer $ \chi(\sigma_{x}=1)=\dfrac{1}{\sqrt{2}}\left[1 \\ 1\right],\quad 		\chi(\sigma_{x}=-1)=\dfrac{1}{\sqrt{2}}\left[1 \\ -1\right] $

		$ \chi(\sigma_{y}=1)=\dfrac{1}{\sqrt{2}}\left[1 \\ i\right],\quad \chi(\sigma_{y}=-1)=\dfrac{1}{\sqrt{2}}\left[1 \\ -i\right] $

% 3
\answer $ \sigma_{n}=\begin{bmatrix}
	\cos\theta & \sin\theta e^{-i\varphi} \\
	\sin\theta e^{i\varphi} & -\cos\theta
\end{bmatrix}=\begin{bmatrix}
	n_{z} & n_{x}-in_{y} \\ n_{x}+in_{y} & -n_{z}
\end{bmatrix} $

	$ \chi(\sigma_{n}=1)=\begin{bmatrix}
		\cos\dfrac{\theta}{2} \\ \sin\dfrac{\theta}{2}e^{i\varphi}
	\end{bmatrix},\dfrac{1}{\sqrt{2(1+n_{z})}}\begin{bmatrix}
		1+n_{z} \\ n_{x}+in_{y}
\end{bmatrix} $
	
	或$ \dfrac{1}{\sqrt{2}(1-n_{z})}\begin{bmatrix}
		n_{x}-in_{y} \\ 1-n_{z}
	\end{bmatrix} $
	
	$ \chi(\sigma_{n}=-1)=\begin{bmatrix}
		\sin\dfrac{\theta}{2} \\ -\cos\dfrac{\theta}{2}e^{i\varphi}
	\end{bmatrix},\dfrac{1}{\sqrt{2(1+n_{z})}}\begin{bmatrix}
		n_{x}-in_{y} \\ -(1+n_{z})
	\end{bmatrix} $
	
	或$ \dfrac{1}{\sqrt{2}(1-n_{z})}\begin{bmatrix}
		1-n_{z} \\ -(n_{x}+in_{y})
	\end{bmatrix} $

% 4
\answer $ \sigma_{n}=1,\langle\boldsymbol{\sigma}\rangle=\boldsymbol{n}.\quad \sigma_{n}=-1,\quad \langle\boldsymbol{\sigma}\rangle=-\boldsymbol{n} $

		$ \Delta S_{x}=\sqrt{1-n_{x}^{2}}\dfrac{\hbar}{2},\quad \Delta S_{y}=\sqrt{1-n_{y}^{2}}\dfrac{\hbar}{2},\quad \Delta S_{z}=\sqrt{1-n_{z}^{2}}\dfrac{\hbar}{2} $

\stepcounter{answer}

% 6
\answer  $ (1+\sigma_{x})^{\frac{1}{2}}=\dfrac{1}{\sqrt{2}}(1+\sigma_{x}),\quad (1+\sigma_{x})^{-1} $ 不存在 

		$ (1+\sigma_{x}+i\sigma_{y})^{\frac{1}{2}}=1+\dfrac{1}{2}(\sigma_{x}+i\sigma_{y}) $

\stepcounter{answer}	\stepcounter{answer}

% 9
\answer $ T_{r}(\boldsymbol{A}\cdot\boldsymbol{\sigma})=0,\quad T_{r}[(\boldsymbol{A}\cdot\boldsymbol{\sigma})(\boldsymbol{B}\cdot\boldsymbol{\sigma})=2\boldsymbol{A}\times\boldsymbol{B}] $

		$ T_{r}[(\boldsymbol{A}\cdot\boldsymbol{\sigma})(\boldsymbol{B}\cdot\boldsymbol{\sigma})(\boldsymbol{C}\cdot\boldsymbol{\sigma})]=2i\boldsymbol{A}\cdot(\boldsymbol{B}\times\boldsymbol{C})=2i(\boldsymbol{A}\times\boldsymbol{B})\cdot\boldsymbol{C} $

\stepcounter{answer}	\stepcounter{answer}	\stepcounter{answer}	\stepcounter{answer}	

% 14
\answer $ \Lambda_{l}^{+}+\Lambda_{l}^{-}=1,\quad \Lambda_{l}^{+}\Lambda_{l}^{-}=\Lambda_{l}^{-}\Lambda_{l}^{+}=0,\quad (\Lambda_{l}^{+})^{2}=\Lambda_{l}^{+},\quad (\Lambda_{l}^{-})^{2}=\Lambda_{l}^{-} $

		当$ j=l+\dfrac{1}{2},\quad \Lambda_{l}^{+}\varPsi_{ljm_{j}}=\varPsi_{ljm_{j}},\quad \Lambda_{l}^{-}=0 $
		
		当$ j=l-\dfrac{1}{2},\quad \Lambda_{l}^{+}\varPsi_{ljm_{j}}=0,\quad \Lambda_{l}^{-}=\varPsi_{ljm_{j}} $

\stepcounter{answer}

% 16
\answer $ \dfrac{\langle ljj|\mu_{z}|ljj \rangle }{\mu_{B}}=-gj=\begin{dcases}
	-\left(j+\dfrac{1}{2}\right),\quad j=l+\dfrac{1}{2}	\\
	-\dfrac{j(2j+1)}{2j+2},\quad j=l-\dfrac{1}{2}
\end{dcases} $

% 17
\answer $ J_{x}=\dfrac{\hbar}{2}.\quad \langle\boldsymbol{J}^{2}\rangle=\left[l(l+1)+\dfrac{3}{4}\right]\hbar^{2} $

		$ \boldsymbol{J}^{2}=\left(l+\dfrac{1}{2}\right)\left(l+\dfrac{3}{2}\right)\hbar^{2}$的概率为$\dfrac{(l+1)}{2l+1}, $
		
		$ \boldsymbol{J}^{2}=\left(l-\dfrac{1}{2}\right)\left(l+\dfrac{1}{2}\right)\hbar^{2}$的概率为$\dfrac{l}{2l+1} $

% 18
\answer (a)$ [\hat{v}_{x},\hat{v}_{y}]=\dfrac{i\hbar qB}{m^{2}c},\quad [\hat{v}_{x},\hat{v}_{z}]=0,\quad [\hat{v}_{y},\hat{v}_{z}]=0 $

		(b)$ \hat{Q}=m\sqrt{\dfrac{c}{\hbar qB}}\hat{v}_{x},\quad \hat{P}=m\sqrt{\dfrac{c}{\hbar qB}}\hat{v}_{y} $
		
		(c)$ E=\left(n+\dfrac{1}{2}\right)\hbar\omega+\dfrac{\hbar^{2}k^{2}}{2m_{c}},\quad, \omega=\dfrac{|q|B}{mc} $
		
\aindent$ n=0,1,2,\cdots\quad -\infty<k<\infty $

% 19
\answer $ H=\dfrac{1}{2\mu}(\hat{p_{x}}^{2}+\hat{p_{y}}^{2}+\hat{p_{z}}^{2})+\dfrac{q^{2}B^{2}}{8\mu c^{2}}(x^{2}+y^{2})-\dfrac{qB}{2\mu c}\hat{L_{z}} $

		$ E=(2n_{\rho}+1+|m|)\hbar|\omega|-m\hbar\omega+\dfrac{\hbar^{2}k^{2}}{2\mu} $
		
\aindent$ =(2n_{\rho}+1+|m|\mp m)\dfrac{\hbar|q|B}{2\mu c}+\dfrac{\hbar^{2}k^{2}}{2\mu} $
		
		$ L_{z}=m\hbar,\quad p_{z}=\hbar k,\quad \omega=\dfrac{qB}{2\mu c} $
		
		$ m=0,\pm1,\pm2,\cdots,\quad n_{\rho}=0,1,2,\cdots\quad -\infty<k<\infty $

% 20
\answer $ a(t)=\cos\omega t,\quad b(t)=-i\sin\omega t,\quad \omega=\dfrac{eB}{2m_{e}c} $

		$ \bar{S_{x}}(t)=0,\quad \bar{S_{y}}(t)=-\dfrac{\hbar}{2}\sin\omega t,\quad \bar{S_{z}}(t)=\dfrac{\hbar}{2}\cos\omega t $

\stepcounter{answer}

% 22
\answer $ \Delta E_{nl}=\dfrac{ \frac{\e^{2}}{a_{0}}\left(\frac{\e^{2}}{\hbar c}\right) }{2l(l+1)n^{3}}(l\neq0) $

% 23
\answer $ \boldsymbol{S}^{2}=0.2\hbar^{2}, $概率均为$\dfrac{1}{2}$

% 24
\answer $ \chi=\dfrac{1}{\sqrt{2}}\chi_{11}+\dfrac{1}{2}(\chi_{10}+\chi_{00}) $

		$ \boldsymbol{S}^{2}=0,2\hbar^{2}, $概率为$\dfrac{1}{4},\dfrac{3}{4}$
		
		$ S_{z}=0,\hbar, $概率为$\dfrac{1}{2},\dfrac{1}{2}$

% 25
\answer $ \boldsymbol{S}^{2}=S(S+1)\hbar^{2},\quad S=\dfrac{3}{2},\dfrac{1}{2} $

		$ E=\dfrac{3\hbar\omega_{0}}{4}, $简并度4;\quad $E=-\dfrac{3\hbar\omega_{0}}{4},$简并度4

% 26
\answer $ \varPsi_{22}=\alpha(1)\alpha(2) $

		$ \varPsi_{21}=\dfrac{1}{\sqrt{2}}[\alpha(1)\beta(2)+\beta(1)\alpha(2)] $
		
		$ \varPsi_{20}=\dfrac{1}{\sqrt{6}}[\alpha(1)\gamma(2)+2\beta(1)\beta(2)+\gamma(1)\alpha(2)] $
		
		$ \varPsi_{2-1}=\dfrac{1}{\sqrt{2}}[\beta(1)\gamma(2)+\gamma(1)\beta(2)] $
		
		$ \varPsi_{2-2}=\gamma(1)\gamma(2) $
		
		$ \varPsi_{11}=\dfrac{1}{\sqrt{2}}[\alpha(1)\beta(2)-\beta(1)\alpha(2)] $
		
		$ \varPsi_{10}=\dfrac{1}{\sqrt{2}}[\alpha(1)\gamma(2)-\gamma(1)\alpha(2)] $
		
		$ \varPsi_{1-1}=\dfrac{1}{\sqrt{2}}[\beta(1)\gamma(2)-\gamma(1)\beta(2)] $
		
		$ \varPsi_{00}=\dfrac{1}{\sqrt{3}}[\alpha(1)\gamma(2)-\beta(1)\beta(2)+\gamma(1)\alpha(2)] $


\stepcounter{answer}	\stepcounter{answer}

% 29
\answer $ -\boldsymbol{a}\cdot\boldsymbol{b} $