\achapter
% \stepcounter{answer}

% 1
\answer $ \boldsymbol{L}^{2},L_{x}$ 共同本征态

	$ Z_{11}=\dfrac{1}{2}Y_{11}+\dfrac{1}{\sqrt{2}}Y_{10}+\dfrac{1}{2}Y_{1-1} $

	$ Z_{10}=\dfrac{1}{\sqrt{2}}(Y_{11}-Y_{1-1}) $

	$ Z_{1-1}=\dfrac{1}{2}Y_{11}-\dfrac{1}{\sqrt{2}}Y_{10}+\dfrac{1}{2}Y_{1-1} $

	$ \boldsymbol{L}^{2},L_{y}$ 共同本征态
	
	$ X_{11}=\dfrac{1}{2}Y_{11}+\dfrac{i}{\sqrt{2}}Y_{10}-\dfrac{1}{2}Y_{1-1} $

	$ X_{10}=\dfrac{1}{\sqrt{2}}(Y_{11}+Y_{1-1}) $

	$ X_{1-1}=\dfrac{1}{2}Y_{11}-\dfrac{i}{\sqrt{2}}Y_{10}-\dfrac{1}{2}Y_{1-1} $

% 2
\answer $Y_{10}$态$(L_{x}=\hbar),\bar{L_{x}^{2}}=\hbar^{2},\quad L_{x}=\pm\hbar,\quad $ 没有$L_{x}=0$本征态成分

% 3
\answer (a) $Y_{11}=\dfrac{1}{2}(Z_{11}+Z_{1-1})+\dfrac{1}{\sqrt{2}}Z_{10}$

\aindent $ L_{x}=\hbar,0,-\hbar \quad$ 概率$w_{1}=\dfrac{1}{4},\quad w_{0}=\dfrac{1}{2},\quad w_{-1}=\dfrac{1}{4}$ 

		(b) $Y_{11}$态$\bar{L_{x}}=0,\quad \bar{L_{x}^{2}}=\dfrac{\hbar^{2}}{2}$
		
\aindent $ w_{1}-w_{-1}=0,\quad w_{1}+w_{-1}=\dfrac{1}{2},\quad $解出$w_{1}=w_{-1}=\dfrac{1}{4},\quad w_{0}=\dfrac{1}{2} $

% 4
\answer (a) $2\hbar^{2}\qquad$ (b) 0\qquad (c)$ \dfrac{1}{6} $

		(d) $L_{z}=0,$概率$\dfrac{1}{6};$\quad $L_{x}=\pm\hbar,$概率各为$\dfrac{5}{12}$

% 5
\answer $ E\sim\dfrac{\mu\e^{4}}{2\hbar^{2}} $

% 6
\answer $ E\sim\dfrac{0.84\mu^{3}\lambda^{4}}{\hbar^{6}} $

\stepcounter{answer}

% 8
\answer $ \Delta x_{0}=a_{0},\quad \Delta p_{x}=\dfrac{\hbar}{\sqrt{3}a_{0}} $

% 9
\answer $ 13\times e^{-4}=\num{0.2381} $

% 10
\answer $ w_{n}=\left[1+4n+\dfrac{(4n)^{2}}{2!}+\cdots+\dfrac{(4n)^{2n}}{(2n)!}\right]e^{-4n} $

	$ w_{1}=\num{0.2381},\quad w_{2}=\num{0.0996},\quad w_{3}=\num{0.0458}, $
	
	$ w_{4}=\num{0.0220},\quad w_{5}=\num{0.0108} $

% 11
\answer $ r_{\text{概}}=n^{2}a_{0},\quad \bar{r}=\left(n^{2}+\dfrac{n}{2}\right)a_{0},\quad \bar{r^{2}}=n^{2}\left(n+\dfrac{1}{2}\right)(n+1)a_{0}^{2} $

	$ \Delta r=(\bar{r^{2}}-\bar{r}^{2})^{\frac{1}{2}}=n\sqrt{\dfrac{n}{2}+\dfrac{1}{4}a_{0}},\quad \dfrac{\Delta r}{\bar{r}}=\dfrac{1}{\sqrt{2n+1}} $

% 12
\answer $ \bigg|\int\varPsi_{100}(Z+1,r)\varPsi_{100}(Z,r)d\tau \bigg|^{2}=\dfrac{Z^{3}(Z+1)^{3}}{\left(Z+\dfrac{1}{2}\right)^{6}} $

% 13
\answer $ E=-\dfrac{\e^{2}}{2a_{0}}(n_{r}+l^{\prime}+1)^{-2},\quad l^{\prime}\approx l-\dfrac{\lambda}{\left(l+\dfrac{1}{2}\right)}=l-\delta_{l} $

\stepcounter{answer}

% 15
\answer $ \langle\dfrac{1}{r}\rangle=\dfrac{Z}{n^{2}a_{0}},\quad \langle\dfrac{1}{r^{2}}\rangle=\dfrac{Z^{2}}{n^{3}\left(l+\dfrac{1}{2}\right)a_{0}^{2}},\quad \langle\dfrac{1}{r^{3}}\rangle=\dfrac{Z^{3}}{n^{3}l\left(l+\dfrac{1}{2}\right)(l+1)a_{0}^{3}} $

% 16
\answer 条件$ \lambda>-(2l+1) $

% 17
\answer $ \bar{r}=\dfrac{1}{2}[3n^{2}-l(l+1)]\dfrac{a_{0}}{2},\quad \bar{r^{2}}=\dfrac{1}{2}n^{2}[5n^{2}+1-3l(l+1)]\dfrac{a_{0}^{2}}{Z^{2}} $

% 18
\answer $ \Delta x=\dfrac{a_{0}n\sqrt{5n^{2}+1}}{\sqrt{6}},\quad \Delta p_{x}=\dfrac{\hbar}{\sqrt{3}na_{0}} $

% 19
\answer $ r_{l}=\dfrac{l(l+1)a_{0}}{Z},\quad V_{l}(r_{l})=-\dfrac{Z\e^{2}}{2r_{l}} $

	$ V_{l}(r)\approx V_{l}(r_{l})+\dfrac{1}{2}\mu\omega_{l}^{2}(r-r_{l})^{2},\quad \omega_{l}^{2}=\dfrac{Z\e^{2}}{\mu r_{l}^{3}} $
	
	$ E\approx V_{l}(r_{l})+\left(n_{r}+\dfrac{1}{2}\right)\hbar\omega_{l},\quad n_{r}=0,1,2,\cdots $

% 20
\answer $ F(\xi)=F(-n_{\rho},|m|+1,\xi),\quad E_{N}=(N+1)\hbar\omega=(2n_{\rho}+|m|+1)\hbar\omega $

% 21
\answer $ F(\xi)=F\left(-n_{r},l+\dfrac{3}{2},\xi\right),\quad E_{N}=\left(N+\dfrac{3}{2}\right)\hbar\omega,\quad N=l+2n $

% 22
\answer 二维谐振子$E_{N}$简并度$(N+1)$； 三维谐振子$E_{N}$简并度$\dfrac{1}{2}(N+1)( N+2)$

% 23
\answer $ r_{\text{概}}=\dfrac{1}{\alpha},\quad \bar{r}=\dfrac{2}{\sqrt{\pi}\alpha},\quad \Delta r=\dfrac{\sqrt{\dfrac{3}{2}}-\dfrac{4}{\pi}}{\alpha},\quad \dfrac{1}{\alpha}=\sqrt{\dfrac{\hbar}{\mu\omega}} $

% 24
\answer $ \hbar\omega\dfrac{l(l+1)}{2I+1} $，与$n_{r}$无关.